src/canonize/test.lean
@@ -2,7 +2,7 @@ import .term .tactic
 
 open tactic polya polya.term
 
--- build term and proove equality
+-- build term and prove equality
 meta def test (e : expr) : tactic unit :=
 do
     (_, pr) ← nterm_of_expr e,
@@ -17,6 +17,6 @@ set_option profiler true
 set_option trace.app_builder true
 
 run_cmd test `(x * y + 1 * x + 0 * (z + y))
-run_cmd test `(x + x)
+run_cmd test `(x / x)
 run_cmd test `(x * 2)
 run_cmd test `(x * (2 : γ))
